WIP: Update examples

io/ho_examples/Callback.Example.fst
@@ -26,17 +26,23 @@ type cb  = fd:file_descr -> IIO (maybe bool) (fun h -> is_open fd h) (fun h _ lt
 type ctx = cb:cb         -> IIO (maybe unit) (fun _ -> True)           (fun h r lt -> enforced_locally pi h lt)
 type pp  = f: ctx        -> IIO (maybe unit) (fun _ -> True)           (fun h r lt -> enforced_locally pi h lt)
 
-let cb_mlifyable : mlifyable cb = 
+let cb_monitorable_hist : monitorable_hist (fun fd h -> is_open fd h) (fun fd h (x:maybe bool) lt -> lt == []) pi = {
+  c1post = admit ()
+}
+
+let cb_mlifyable : mlifyable cb pi = 
   mlifyable_iiowp_trivialize_weaken_post
     file_descr
     bool
     (fun fd h -> is_open fd h)
     (fun fd h _ lt -> lt == [])
+    pi
+    #cb_monitorable_hist
+    
 
 let cb_mlifyable_in : mlifyable_in_arr1 file_descr bool (fun fd h -> is_open fd h) (fun fd h r lt -> lt == []) pi = {
   ca1 = importable_safe_importable file_descr;
   cmlifyable1 = cb_mlifyable;
-  cpi1 = ()
 }
 
 private
@@ -46,28 +52,34 @@ private
 let lemma_c2post () : squash (forall h lt. enforced_locally pi h lt  ==> enforced_locally pi h lt) =
   lemma_c1post ()
 
-let pp_post_monitorable : monitorable_hist (fun fd h -> True) (fun fd h r lt -> enforced_locally pi h lt) pi = {
+let pp_post_monitorable : checkable_hist_post (fun fd h -> True) (fun fd h r lt -> enforced_locally pi h lt) pi = {
+  cmonitorable = {
+    c1post = lemma_c1post ();
+  };
   result_check = (fun _ _ _ _ -> true);
-  c1post = lemma_c1post ();
   c2post = lemma_c2post ();
 }
 
+unfold
 let ctx_instrumentable : instrumentable ctx pi =
-  instrumentable_HO_arr1_out_importable file_descr bool (fun fd h -> is_open fd h) (fun fd h r lt -> lt == []) unit (fun h -> True) (fun h r lt -> enforced_locally pi h lt) pi
-  #(importable_safe_importable _ #(safe_importable_ml (maybe unit) #(mlfo_maybe unit #(ML_FO mlfo_unit))))
-  #cb_mlifyable_in
-  #pp_post_monitorable
+  instrumentable_HO_arr1_out_importable
+    file_descr bool (fun fd h -> is_open fd h) (fun fd h r lt -> lt == []) 
+    unit (fun h -> True) (fun h r lt -> enforced_locally pi h lt) 
+    pi
+    #(importable_safe_importable _ #(safe_importable_ml (maybe unit) #(mlfo_maybe unit #(ML_FO mlfo_unit))))
+    #cb_mlifyable_in
+    #pp_post_monitorable
   
-let pp_mlifyable : mlifyable pp =
+let pp_mlifyable : mlifyable pp (trivial_pi ()) =
   mlifyable_inst_iiowp_weaken ctx #ctx_instrumentable (maybe unit) (fun h r lt -> enforced_locally pi h lt)
 
 let main : pp = fun c ->
   let theCb : cb = fun fd -> if is_open fd (get_trace ()) then Inl true else Inl false in
   c theCb
 
-(** I can not write a context in the intermediate language because the type of the callback is not informative 
-    enough to know it respects pi. **)
-let c (theCb : file_descr -> MIIO (maybe bool)) : IIOpi (maybe unit) pi =
+val c : ctx_instrumentable.inst_type
+//let c (theCb : file_descr -> IIOpi (maybe bool) pi) : IIOpi (maybe unit) pi =
+let c (theCb : cb_mlifyable.matype) : IIOpi (maybe unit) pi =
   let fd = static_cmd Openfile "/tmp2/passwd" in
   if Inl? fd  then
     let test = theCb (Inl?.v fd) in
@@ -75,6 +87,6 @@ let c (theCb : file_descr -> MIIO (maybe bool)) : IIOpi (maybe unit) pi =
     else Inr Something_went_really_bad
   else Inr Something_went_really_bad
 
-let main_mlify = mlify #_ #pp_mlifyable main
+let main_mlify = mlify #_ #_ #pp_mlifyable main
 
 let whole () : MIIO (maybe unit) = main_mlify c
